src/CursorList.v
@@ -1,0 +1,84 @@
+(* This file implements, for lack of a better name, a cursor list.
+This is a list for which each element contains a "cursor" type: each
+element is parameterized over a 'from' and 'to' element of this type,
+which must match with the previous element. For that reason this is
+also a snoc list. Note that this is not unlike fhlist from CPDT,
+except we place further restrictions on it. *)
+From SmartContracts Require Import Automation.
+Section CursorList.
+Context {cursor_type : Type} {elm_type : cursor_type -> cursor_type -> Type}.
+
+Inductive CursorList : cursor_type -> cursor_type -> Type :=
+  | nil : forall {elm}, CursorList elm elm
+  | snoc : forall {from mid to}, CursorList from mid -> elm_type mid to -> CursorList from to.
+
+Definition snoc_eq
+           {from mid mid' to}
+           (xs : CursorList from mid)
+           (x : elm_type mid' to) :
+  mid' = mid -> CursorList from to :=
+  fun eq =>
+    snoc xs (match eq with eq_refl => x end).
+
+Fixpoint clist_app
+           {from mid to}
+           (xs : CursorList from mid)
+           (ys : CursorList mid to) : CursorList from to :=
+  match ys with
+  | nil => fun xs => xs
+  | snoc ys' y => fun xs => snoc (clist_app xs ys') y
+  end xs.
+
+Infix "++" := clist_app (right associativity, at level 60).
+
+Definition clist_prefix
+           {from mid to}
+           (prefix : CursorList from mid)
+           (full : CursorList from to) : Prop :=
+  exists suffix, full = prefix ++ suffix.
+
+Definition clist_suffix
+           {from mid to}
+           (suffix : CursorList mid to)
+           (full : CursorList from to) : Prop :=
+  exists prefix, full = prefix ++ suffix.
+
+Infix "`prefix_of`" := clist_prefix (at level 70).
+Infix "`suffix_of`" := clist_suffix (at level 70).
+
+Section Theories.
+Lemma clist_app_nil_l {from to} (xs : CursorList from to) :
+  nil ++ xs = xs.
+Proof. induction xs; auto; cbn; solve_by_rewrite. Qed.
+
+Lemma clist_app_assoc
+      {c1 c2 c3 c4}
+      (xs : CursorList c1 c2)
+      (ys : CursorList c2 c3)
+      (zs : CursorList c3 c4) :
+  xs ++ ys ++ zs = (xs ++ ys) ++ zs.
+Proof. induction zs; intros; auto; cbn; solve_by_rewrite. Qed.
+End Theories.
+
+Lemma prefix_of_app
+      {from mid to to'}
+      {prefix : CursorList from mid}
+      {xs : CursorList from to}
+      {suffix : CursorList to to'} :
+  prefix `prefix_of` xs ->
+  prefix `prefix_of` xs ++ suffix.
+Proof.
+  intros [ex_suffix ex_suffix_eq_app].
+  exists (ex_suffix ++ suffix).
+  rewrite clist_app_assoc; congruence.
+Qed.
+End CursorList.
+
+Delimit Scope clist_scope with trace.
+Bind Scope clist_scope with CursorList.
+Infix "++" := clist_app (right associativity, at level 60) : clist_scope.
+
+Infix "`prefix_of`" := clist_prefix (at level 70) : clist_scope.
+Infix "`suffix_of`" := clist_suffix (at level 70) : clist_scope.
+
+Arguments CursorList : clear implicits.
